lib/steel/pulse/Pulse.Checker.Pure.fst
@@ -383,6 +383,11 @@ let get_non_informative_witness g u t
         T.E_Total
         (non_informative_witness_t u t)
 
+let try_check_prop_validity (g:env) (p:term) (_:tot_typing g p tm_prop)
+  : T.Tac (option (Pulse.Typing.prop_validity g p))
+  = let t_opt, issues = rtb_check_prop_validity g (elab_env g) (elab_term p) in
+    t_opt
+
 let check_prop_validity (g:env) (p:term) (_:tot_typing g p tm_prop)
   : T.Tac (Pulse.Typing.prop_validity g p)
   = let t_opt, issues = rtb_check_prop_validity g (elab_env g) (elab_term p) in
